src/Interpreter/llvm2coq.ml
@@ -1,1 +1,0 @@
-../Parser/llvm2coq.ml
