src/Interpreter/llvm_pretty_printer.ml
@@ -1,1 +1,0 @@
-../Parser/llvm_pretty_printer.ml
