src/Interpreter/ssa_main.ml
@@ -1,1 +1,0 @@
-../ssa/extraction/ssa_main.ml
