src/TV/extraction/coq2llvm.ml
@@ -1,1 +1,0 @@
-../../Parser/coq2llvm.ml
