src/TV/sub_tv_dec.v
@@ -24,13 +24,22 @@ Require Import eq_tv_dec.
 
 Export SimpleSE.
 
+Lemma typ_sterm_dec : forall (st1 st2:typ*sterm), {st1=st2}+{~st1=st2}.
+Proof.
+  destruct st1 as (t1,s1).
+  destruct st2 as (t2,s2).
+  destruct (@typ_dec t1 t2); subst; try solve [done_right].
+  destruct (@sterm_dec s1 s2); subst; try solve [auto | done_right].
+Qed.
+
 Definition sub_sstate s1 s2 := 
   s1.(STerms) <<<= s2.(STerms) /\ s1.(SMem) = s2.(SMem) /\
   s1.(SFrame) = s2.(SFrame) /\ s1.(SEffects) = s2.(SEffects).
 
 Notation "s1 <<= s2" := (sub_sstate s1 s2) (at level 70, no associativity).
 
-Lemma smap_sub_dec : forall (sm1 sm2:smap), uniq sm1 -> {sm1 <<<= sm2}+{~sm1 <<<= sm2}.
+Lemma smap_sub_dec : forall (sm1 sm2:smap), 
+  uniq sm1 -> {sm1 <<<= sm2}+{~sm1 <<<= sm2}.
 Proof.
   induction sm1.  
     intros. left. intros i i_in_nil. fsetdec. 
@@ -45,7 +54,8 @@ Proof.
           left. simpl_env.
           apply subAL_app1; auto.
             intros i Hi_in_dom. simpl in *.
-            destruct (@eq_dec atom (EqDec_eq_of_EqDec atom EqDec_atom) i id); subst.
+            destruct (@eq_dec atom (EqDec_eq_of_EqDec atom EqDec_atom) i id); 
+              subst.
               rewrite <- HeqLookup; auto.
               fsetdec.
 
@@ -55,7 +65,8 @@ Proof.
             assert (id0=id) as Eq. simpl in Hid0_in. fsetdec.
             subst.
             simpl. 
-            destruct (@eq_dec atom (EqDec_eq_of_EqDec atom EqDec_atom) id id); auto.
+            destruct (@eq_dec atom (EqDec_eq_of_EqDec atom EqDec_atom) id id); 
+              auto.
               contradict n; auto.
         right. intro J. assert (H:=@J id). simpl in H.
         destruct (@eq_dec atom (EqDec_eq_of_EqDec atom EqDec_atom) id id); auto.
@@ -70,15 +81,52 @@ Qed.
 Lemma sstate_sub_dec : forall (sts1 sts2:sstate), 
   uniq sts1.(STerms) -> {sts1<<=sts2} + {~sts1<<=sts2}.
 Proof.
-Ltac done_right := 
+Ltac done_right' := 
   right; intro J ; destruct J as [ J1 [J2 [J3 J4]]]; simpl in *; auto.
 
   intros sts1 sts2 Huniq.
   destruct sts1 as [st1 sm1 sf1 se1].
   destruct sts2 as [st2 sm2 sf2 se2].
-  destruct (@sterms_dec se1 se2); subst; try solve [auto | done_right].
-  destruct (@sframe_dec sf1 sf2); subst; try solve [auto | done_right].
-  destruct (@smem_dec sm1 sm2); subst; try solve [auto | done_right].
-  destruct (@smap_sub_dec st1 st2 Huniq); subst; try solve [left; split; auto | done_right].
+  destruct (@sterms_dec se1 se2); subst; try solve [auto | done_right'].
+  destruct (@sframe_dec sf1 sf2); subst; try solve [auto | done_right'].
+  destruct (@smem_dec sm1 sm2); subst; try solve [auto | done_right'].
+  destruct (@smap_sub_dec st1 st2 Huniq); subst; 
+    try solve [left; split; auto | done_right'].
 Qed.
 
+Definition prefix A (l1 l:list A) := exists l2, l1 ++ l2 = l.
+
+(* A more general way is to check if l1 is a subset of l2. By doing that way,
+ * at call-site, we also need to ensure parameters are matched. The prefix
+ * checking is sufficient to Softbound.
+*)
+Lemma prefix_dec : forall A, (forall (a1 a2:A), {a1=a2}+{~a1=a2}) ->
+  forall (l1 l2:list A), {prefix _ l1 l2}+{~prefix _ l1 l2}.
+Proof.
+  induction l1.
+    left. exists l2. auto.
+
+    destruct l2.
+      right. intro J. destruct J as [l EQ].
+      inversion EQ.
+
+      destruct (@X a a0); subst.
+        destruct (@IHl1 l2).
+          left. destruct p as [l EQ]; subst.
+          exists l. auto.
+
+          right. intro J. apply n.
+          destruct J as [l EQ].
+          inversion EQ; subst.
+          exists l. auto.
+        right. intro J. destruct J as [l EQ].        
+        inversion EQ; subst; auto.
+Qed.
+
+(*****************************)
+(*
+*** Local Variables: ***
+*** coq-prog-name: "coqtop" ***
+*** coq-prog-args: ("-emacs-U" "-I" "~/SVN/sol/vol/src/ssa/monads" "-I" "~/SVN/sol/vol/src/ssa/ott" "-I" "~/SVN/sol/vol/src/ssa/compcert" "-I" "~/SVN/sol/theory/metatheory_8.3") ***
+*** End: ***
+ *)
