src/ssa/ssa_interpreter.v
@@ -1,0 +1,489 @@
+Add LoadPath "./ott".
+Add LoadPath "./monads".
+Add LoadPath "./compcert".
+(* Add LoadPath "../../../theory/metatheory". *)
+
+Require Import ssa_dynamic.
+Require Import trace.
+Require Import Metatheory.
+Require Import assoclist.
+Require Import monad.
+Require Import genericvalues.
+Require Import ssa_mem.
+Require Import Values.
+Require Import Memory.
+Require Import Integers.
+Require Import Coqlib.
+Require Import ssa_props.
+
+Export LLVMopsem.
+
+Definition interInsn (state:State) : option (State*trace) :=
+(* Check if the stack is empty. *) 
+match state with
+| mkState Sys TD Ps nil gl fs Mem0 => None
+| mkState Sys TD Ps ((mkEC F B cs tmn lc arg0 als)::EC) gl fs Mem0 =>
+  (* If cs is nil, we check tmn, 
+     otherwise, we check the first cmd in cs *)
+  match cs with
+  | nil => (* terminator *)
+    match tmn with
+    | insn_return rid RetTy Result =>
+      (* the suspended stacks cannot be empty, and
+          there must be a caller of the current function. *)
+      match EC with
+      | nil => None
+      | (mkEC F' B' nil tmn' lc' arg' als')::EC'' => None
+      | (mkEC F' B' (c'::cs') tmn' lc' arg' als')::EC'' =>
+        (* there must be a caller of the current function. *)
+        if (Instruction.isCallInst c') 
+        then 
+          do Mem' <- free_allocas TD Mem0 als;
+             ret ((mkState Sys TD Ps ((mkEC F' B' cs' tmn' (returnUpdateLocals TD c' RetTy Result lc lc' gl) arg' als')::EC'') gl fs Mem'),
+                  trace_nil)
+        else None
+      end
+    | insn_return_void rid =>
+      (* the suspended stacks cannot be empty, and
+          there must be a caller of the current function. *)
+      match EC with
+      | nil => None
+      | (mkEC F' B' nil tmn' lc' arg' als')::EC'' => None
+      | (mkEC F' B' (c'::cs') tmn' lc' arg' als')::EC'' =>
+        (* there must be a caller of the current function. *)
+        if (Instruction.isCallInst c')
+        then
+          do Mem' <- free_allocas TD Mem0 als;
+             ret ((mkState Sys TD Ps ((mkEC F' B' cs' tmn' lc' arg' als')::EC'') gl fs Mem'),
+                  trace_nil)
+        else None
+      end
+    | insn_br bid Cond l1 l2 =>
+      (* read the value of Cond *)
+      do cond0 <- (getOperandValue TD Cond lc gl);
+      (* look up the target block *)
+        match (if isGVZero TD cond0
+               then lookupBlockViaLabelFromFdef F l2
+               else lookupBlockViaLabelFromFdef F l1) with
+        | None => None
+        | Some (block_intro l' ps' cs' tmn') =>
+            Some ((mkState Sys TD Ps ((mkEC F (block_intro l' ps' cs' tmn') cs' tmn' 
+                     (switchToNewBasicBlock TD (block_intro l' ps' cs' tmn') B gl lc) arg0 als)::EC) gl fs Mem0),
+                  trace_nil)
+        end
+    | insn_br_uncond bid l0 =>
+      (* look up the target block *)
+      match (lookupBlockViaLabelFromFdef F l0) with
+      | None => None
+      | Some (block_intro l' ps' cs' tmn') =>
+          Some ((mkState Sys TD Ps ((mkEC F (block_intro l' ps' cs' tmn') cs' tmn' 
+                        (switchToNewBasicBlock TD (block_intro l' ps' cs' tmn') B gl lc) arg0 als)::EC) gl fs Mem0),
+               trace_nil)
+      end
+    | insn_unreachable _ => None
+    end
+
+  | c::cs => (* non-terminator *)
+    match c with
+    | insn_bop id0 bop0 sz0 v1 v2 => 
+      do gv3 <- BOP TD lc gl bop0 sz0 v1 v2;
+         ret ((mkState Sys TD Ps ((mkEC F B cs tmn (updateAddAL _ lc id0 gv3) arg0 als)::EC) gl fs Mem0),
+              trace_nil)         
+    | insn_fbop id0 fbop0 fp0 v1 v2 => 
+      do gv3 <- FBOP TD lc gl fbop0 fp0 v1 v2;
+         ret ((mkState Sys TD Ps ((mkEC F B cs tmn (updateAddAL _ lc id0 gv3) arg0 als)::EC) gl fs Mem0),
+              trace_nil)         
+    | insn_extractvalue id0 t v idxs =>
+      do gv <- getOperandValue TD v lc gl;
+      do gv' <- extractGenericValue TD t gv idxs;
+         ret ((mkState Sys TD Ps ((mkEC F B cs tmn (updateAddAL _ lc id0 gv') arg0 als)::EC) gl fs Mem0),
+              trace_nil)
+    | insn_insertvalue id0 t v t' v' idxs =>
+      do gv <- getOperandValue TD v lc gl;
+      do gv' <- getOperandValue TD v' lc gl;
+      do gv'' <- insertGenericValue TD t gv idxs t' gv';
+         ret ((mkState Sys TD Ps ((mkEC F B cs tmn (updateAddAL _ lc id0 gv'') arg0 als)::EC) gl fs Mem0),
+             trace_nil)
+    | insn_malloc id0 t v0 align0 =>
+      do tsz <- getTypeAllocSize TD t;
+      do gn <- getOperandValue TD v0 lc gl;
+      match (malloc TD Mem0 tsz gn align0) with
+      | None => None
+      | Some (Mem', mb) =>
+        ret ((mkState Sys TD Ps ((mkEC F B cs tmn (updateAddAL _ lc id0 (blk2GV TD mb)) arg0 als)::EC) gl fs Mem'),
+            trace_nil)
+      end
+    | insn_free fid t v =>
+      do mptr <- getOperandValue TD v lc gl;
+      do Mem' <- free TD Mem0 mptr;
+         ret ((mkState Sys TD Ps ((mkEC F B cs tmn lc arg0 als)::EC) gl fs Mem'), trace_nil)
+    | insn_alloca id0 t v0 align0 =>
+      do tsz <- getTypeAllocSize TD t;
+      do gn <- getOperandValue TD v0 lc gl;
+      match (malloc TD Mem0 tsz gn align0) with
+      | None => None
+      | Some (Mem', mb) =>
+          ret ((mkState Sys TD Ps ((mkEC F B cs tmn (updateAddAL _ lc id0 (blk2GV TD mb)) arg0 (mb::als))::EC) gl fs Mem'),
+              trace_nil)
+      end
+    | insn_load id0 t v align0 =>
+      do mp <- getOperandValue TD v lc gl;
+      do gv <- mload TD Mem0 mp t align0;
+         ret ((mkState Sys TD Ps ((mkEC F B cs tmn (updateAddAL _ lc id0 gv) arg0 als)::EC) gl fs Mem0),
+              trace_nil)
+    | insn_store sid t v1 v2 align0 =>
+      do gv1 <- getOperandValue TD v1 lc gl;
+      do mp2 <- getOperandValue TD v2 lc gl;
+      do Mem' <- mstore TD Mem0 mp2 t gv1 align0;
+         ret ((mkState Sys TD Ps ((mkEC F B cs tmn lc arg0 als)::EC) gl fs Mem'),
+             trace_nil)
+    | insn_gep id0 inbounds0 t v idxs =>
+      do mp <- getOperandValue TD v lc gl;
+      do vidxs <- values2GVs TD idxs lc gl;
+      do mp' <- GEP TD t mp vidxs inbounds0;
+         ret ((mkState Sys TD Ps ((mkEC F B cs tmn (updateAddAL _ lc id0 mp') arg0 als)::EC) gl fs Mem0),
+             trace_nil)
+    | insn_trunc id0 truncop0 t1 v1 t2 =>
+      do gv2 <- TRUNC TD lc gl truncop0 t1 v1 t2;
+         ret ((mkState Sys TD Ps ((mkEC F B cs tmn (updateAddAL _ lc id0 gv2) arg0 als)::EC) gl fs Mem0),
+             trace_nil)
+    | insn_ext id0 extop0 t1 v1 t2 =>
+      do gv2 <- EXT TD lc gl extop0 t1 v1 t2;
+         ret ((mkState Sys TD Ps ((mkEC F B cs tmn (updateAddAL _ lc id0 gv2) arg0 als)::EC) gl fs Mem0),
+             trace_nil)
+    | insn_cast id0 castop0 t1 v1 t2 =>
+      do gv2 <- CAST TD lc gl castop0 t1 v1 t2;
+         ret ((mkState Sys TD Ps ((mkEC F B cs tmn (updateAddAL _ lc id0 gv2) arg0 als)::EC) gl fs Mem0),
+             trace_nil)
+    | insn_icmp id0 cond0 t v1 v2 =>
+      do gv3 <- ICMP TD lc gl cond0 t v1 v2;
+         ret ((mkState Sys TD Ps ((mkEC F B cs tmn (updateAddAL _ lc id0 gv3) arg0 als)::EC) gl fs Mem0),
+             trace_nil)
+    | insn_fcmp id0 fcond0 fp v1 v2 =>
+      do gv3 <- FCMP TD lc gl fcond0 fp v1 v2;
+         ret ((mkState Sys TD Ps ((mkEC F B cs tmn (updateAddAL _ lc id0 gv3) arg0 als)::EC) gl fs Mem0),
+             trace_nil)
+    | insn_select id0 v0 t v1 v2 =>
+      do cond0 <- getOperandValue TD v0 lc gl;
+      do gv1 <- getOperandValue TD v1 lc gl;
+      do gv2 <- getOperandValue TD v2 lc gl;
+         ret ((mkState Sys TD Ps ((mkEC F B cs tmn (if isGVZero TD cond0 then updateAddAL _ lc id0 gv2 else updateAddAL _ lc id0 gv1) arg0 als)::EC) gl fs Mem0),
+             trace_nil)  
+    | insn_call rid noret0 tailc0 rt fv lp =>
+      (* only look up the current module for the time being, 
+         do not support linkage. *)
+      do fptr <- getOperandValue TD fv lc gl;
+      do fid <- lookupFdefViaGVFromFunTable fs fptr;
+      match (lookupFdefViaIDFromProducts Ps fid) with
+      | None => 
+        match (lookupFdecViaIDFromProducts Ps fid) with
+        | None => None
+        | Some (fdec_intro (fheader_intro rt' fid' la)) =>
+          if id_dec fid fid' then
+            if typ_dec rt rt' then
+              match (callExternalFunction Mem0 fid (params2GVs TD lp lc gl)) with
+              | (oresult, Mem1) =>
+                ret ((mkState Sys TD Ps 
+                      ((mkEC F B cs tmn 
+                         (exCallUpdateLocals noret0 rid rt oresult
+                            lc) arg0 als)::EC) 
+                       gl fs Mem1),
+                     trace_nil)
+              end
+            else None
+          else None
+        end
+      | Some (fdef_intro (fheader_intro rt' fid' la) lb) =>
+        if id_dec fid fid' then
+          if typ_dec rt rt' then
+            match (getEntryBlock (fdef_intro (fheader_intro rt fid la) lb)) with
+            | None => None
+            | Some (block_intro l' ps' cs' tmn') =>
+                ret ((mkState Sys TD Ps ((mkEC (fdef_intro (fheader_intro rt fid la) lb) 
+                                          (block_intro l' ps' cs' tmn') cs' tmn' (initLocals la (params2GVs TD lp lc gl)) 
+                                          (params2GVs TD lp lc gl) nil)::
+                                        (mkEC F B ((insn_call rid noret0 tailc0 rt fv lp)::cs) tmn lc arg0 als)::EC) gl fs Mem0),
+                    trace_nil)
+            end
+          else None
+        else None
+      end
+    end
+  end
+end.
+
+Lemma dsInsn__implies__interInsn : forall state state' tr,
+  dsInsn state state' tr ->
+  interInsn state = Some (state', tr).
+Proof. 
+  intros state state' tr HdsInsn.
+  Opaque malloc. 
+  (dsInsn_cases (destruct HdsInsn) Case); simpl;
+    try solve [rewrite H; simpl; rewrite H0; simpl; rewrite H1; simpl; auto |
+               rewrite H; simpl; rewrite H0; simpl; auto |
+               rewrite H; simpl; auto ].
+  Case "dsBranch".
+    simpl. rewrite H. simpl. rewrite <- H0. simpl. auto.
+  Case "dsBranch_uncond".
+    simpl. rewrite <- H. simpl. auto.
+  Case "dsCall".
+    unfold lookupFdefViaGV in H.
+    destruct (getOperandValue TD fv lc gl); try solve [inversion H]. simpl.
+    destruct (lookupFdefViaGVFromFunTable fs g); try solve [inversion H]. simpl.
+    rewrite H. simpl in H0. rewrite H0. 
+    apply lookupFdefViaIDFromProducts_ideq in H; subst.
+    destruct (id_dec fid fid); auto.
+      destruct (typ_dec rt rt); auto.
+        contradict n; auto.
+      contradict n; auto.
+  Case "dsExCall".
+    unfold lookupExFdecViaGV in H.
+    destruct (getOperandValue TD fv lc gl); try solve [inversion H]. simpl.
+    destruct (lookupFdefViaGVFromFunTable fs g); try solve [inversion H]. simpl.
+    destruct (lookupFdefViaIDFromProducts Ps i0); try solve [inversion H].
+    rewrite H.
+    apply lookupFdecViaIDFromProducts_ideq in H; subst.
+    rewrite H0. 
+    destruct (id_dec fid fid); auto.
+      destruct (typ_dec rt rt); auto.        
+        contradict n; auto.
+      contradict n; auto.
+Qed.
+
+Lemma interInsn__implies__dsInsn : forall state state' tr,
+  interInsn state = Some (state', tr) ->
+  dsInsn state state' tr.
+Proof.
+  intros state state' tr HinterInsn.
+  destruct state.
+  destruct ECS0; simpl in HinterInsn;
+    try solve [inversion HinterInsn].
+
+    destruct e as [F B cs tmn lc arg0 als].
+    destruct cs.
+      destruct tmn.
+      Case "insn_return".
+        destruct ECS0;
+          try solve [inversion HinterInsn].
+          
+          destruct e as [F' B' cs' tmn' lc' arg' als'].
+          destruct cs';
+            try solve [inversion HinterInsn].
+
+            remember (Instruction.isCallInst c) as R1.
+            remember (free_allocas CurTargetData0 Mem0 als) as R2.
+            destruct R1; try solve [inversion HinterInsn].
+            destruct R2; inversion HinterInsn; subst; eauto.
+
+      Case "insn_return_void".
+        destruct ECS0;
+          try solve [inversion HinterInsn].
+          
+          destruct e as [F' B' cs' tmn' lc' arg' als'].
+          destruct cs';
+            try solve [inversion HinterInsn].
+
+            remember (Instruction.isCallInst c) as R1.
+            remember (free_allocas CurTargetData0 Mem0 als) as R2.
+            destruct R1; try solve [inversion HinterInsn].
+            destruct R2; inversion HinterInsn; subst; eauto.
+
+      Case "insn_br".
+        remember (getOperandValue CurTargetData0 v lc Globals0) as R1.
+        destruct R1; try solve [inversion HinterInsn].
+          simpl in HinterInsn.
+          remember (isGVZero CurTargetData0 g) as R3.
+          destruct R3.
+            remember (lookupBlockViaLabelFromFdef F l1) as R2.
+            destruct R2; inversion HinterInsn; subst.
+              destruct b.
+              inversion HinterInsn; subst.
+              eapply dsBranch; eauto.
+                rewrite <- HeqR3. auto.
+        
+            remember (lookupBlockViaLabelFromFdef F l0) as R2.
+            destruct R2; inversion HinterInsn; subst.
+              destruct b.
+              inversion HinterInsn; subst.
+              eapply dsBranch; eauto.    
+                rewrite <- HeqR3. auto.
+
+      Case "insn_br_uncond".
+        remember (lookupBlockViaLabelFromFdef F l0) as R2.
+        destruct R2; inversion HinterInsn; subst.
+          destruct b.
+          inversion HinterInsn; subst; eauto.
+
+      Case "insn_unreachable".
+        inversion HinterInsn.
+                    
+      destruct c.
+      Case "insn_bop".
+        remember (BOP CurTargetData0 lc Globals0 b s v v0) as R1.
+        destruct R1; 
+          simpl in HinterInsn;
+          inversion HinterInsn; subst; eauto.
+          
+      Case "insn_fbop".
+        remember (FBOP CurTargetData0 lc Globals0 f f0 v v0) as R1.
+        destruct R1; 
+          simpl in HinterInsn;
+          inversion HinterInsn; subst; eauto.
+
+      Case "insn_extractvalue".
+        remember (getOperandValue CurTargetData0 v lc Globals0) as R1.
+        destruct R1; simpl in HinterInsn; 
+          try solve [inversion HinterInsn].         
+        remember (extractGenericValue CurTargetData0 t g l0) as R2.
+        destruct R2; simpl in HinterInsn; 
+          inversion HinterInsn; subst; eauto.
+
+      Case "insn_insertvalue".
+        remember (getOperandValue CurTargetData0 v lc Globals0) as R1.
+        destruct R1; simpl in HinterInsn; 
+          try solve [inversion HinterInsn].         
+        remember (getOperandValue CurTargetData0 v0 lc Globals0) as R2.
+        destruct R2; simpl in HinterInsn; 
+          try solve [inversion HinterInsn].         
+        remember (insertGenericValue CurTargetData0 t g l0 t0 g0) as R3.
+        destruct R3; simpl in HinterInsn; 
+          inversion HinterInsn; subst; eauto.
+          
+      Case "insn_malloc".
+        remember (getTypeAllocSize CurTargetData0 t) as R1.
+        destruct R1; simpl in HinterInsn; 
+          try solve [inversion HinterInsn]. 
+        remember (getOperandValue CurTargetData0 v lc Globals0) as R3.
+        destruct R3; simpl in HinterInsn;
+          try solve [inversion HinterInsn].         
+        remember (malloc CurTargetData0 Mem0 s g a) as R2.
+        destruct R2; simpl in HinterInsn; 
+          try solve [inversion HinterInsn].         
+        destruct p; 
+          inversion HinterInsn; subst; eauto.
+          
+      Case "insn_free".
+        remember (getOperandValue CurTargetData0 v lc Globals0) as R1.
+        destruct R1; simpl in HinterInsn; 
+          try solve [inversion HinterInsn].         
+        remember (free CurTargetData0 Mem0 g) as R2.
+        destruct R2; simpl in HinterInsn; 
+          inversion HinterInsn; subst; eauto.
+          
+      Case "insn_alloca".
+        remember (getTypeAllocSize CurTargetData0 t) as R1.
+        destruct R1; simpl in HinterInsn; 
+          try solve [inversion HinterInsn].         
+        remember (getOperandValue CurTargetData0 v lc Globals0) as R3.
+        destruct R3; simpl in HinterInsn;
+          try solve [inversion HinterInsn].         
+        remember (malloc CurTargetData0 Mem0 s g a) as R2.
+        destruct R2; simpl in HinterInsn; 
+          try solve [inversion HinterInsn].         
+        destruct p; 
+          inversion HinterInsn; subst; eauto.
+          
+      Case "insn_load".
+        remember (getOperandValue CurTargetData0 v lc Globals0) as R1.
+        destruct R1; simpl in HinterInsn; 
+          try solve [inversion HinterInsn].         
+        remember (mload CurTargetData0 Mem0 g t a) as R2.
+        destruct R2; simpl in HinterInsn; 
+          inversion HinterInsn; subst; eauto.
+          
+      Case "insn_store".
+        remember (getOperandValue CurTargetData0 v lc Globals0) as R1.
+        destruct R1; simpl in HinterInsn; 
+          try solve [inversion HinterInsn].         
+        remember (getOperandValue CurTargetData0 v0 lc Globals0) as R2.
+        destruct R2; simpl in HinterInsn; 
+          try solve [inversion HinterInsn].         
+        remember (mstore CurTargetData0 Mem0 g0 t g a) as R3.
+        destruct R3; simpl in HinterInsn; 
+          inversion HinterInsn; subst; eauto.
+          
+      Case "insn_gep".
+        remember (getOperandValue CurTargetData0 v lc Globals0) as R1.
+        destruct R1; simpl in HinterInsn; 
+          try solve [inversion HinterInsn].         
+        remember (values2GVs CurTargetData0 l0 lc Globals0) as R3.
+        destruct R3; simpl in HinterInsn; 
+          try solve [inversion HinterInsn].         
+        remember (GEP CurTargetData0 t g l1 i1) as R2.
+        destruct R2; simpl in HinterInsn; 
+          inversion HinterInsn; subst; eauto.
+
+      Case "insn_trunc".
+        remember (TRUNC CurTargetData0 lc Globals0 t t0 v t1) as R.
+        destruct R; simpl in HinterInsn; 
+          inversion HinterInsn; subst; eauto.
+
+      Case "insn_ext".
+        remember (EXT CurTargetData0 lc Globals0 e t v t0) as R.
+        destruct R; simpl in HinterInsn; 
+          inversion HinterInsn; subst; eauto.
+
+      Case "insn_cast".
+        remember (CAST CurTargetData0 lc Globals0 c t v t0) as R.
+        destruct R; simpl in HinterInsn; 
+          inversion HinterInsn; subst; eauto.
+
+      Case "insn_icmp".
+        remember (ICMP CurTargetData0 lc Globals0 c t v v0) as R.
+        destruct R; simpl in HinterInsn; 
+          inversion HinterInsn; subst; eauto.
+
+      Case "insn_fcmp".
+        remember (FCMP CurTargetData0 lc Globals0 f f0 v v0) as R.
+        destruct R; simpl in HinterInsn; 
+          inversion HinterInsn; subst; eauto.
+
+      Case "insn_select".
+        remember (getOperandValue CurTargetData0 v lc Globals0) as R1.
+        destruct R1; simpl in HinterInsn; 
+          try solve [inversion HinterInsn].         
+        remember (getOperandValue CurTargetData0 v0 lc Globals0) as R2.
+        destruct R2; simpl in HinterInsn; 
+          try solve [inversion HinterInsn].         
+        remember (getOperandValue CurTargetData0 v1 lc Globals0) as R3.
+        destruct R3; simpl in HinterInsn; 
+          try solve [inversion HinterInsn].
+        inversion HinterInsn; subst; eauto.
+
+      Case "insn_call".
+        remember (getOperandValue CurTargetData0 v lc Globals0) as R0.
+        destruct R0; try solve [inversion HinterInsn]. simpl in HinterInsn.
+        remember (lookupFdefViaGVFromFunTable FunTable0 g) as R4.
+        destruct R4; try solve [inversion HinterInsn]. simpl in HinterInsn.
+        remember (lookupFdefViaIDFromProducts CurProducts0 i1) as R1.
+        destruct R1; simpl in HinterInsn.
+          destruct f. destruct f.
+          destruct (id_dec i1 i2); try solve [inversion HinterInsn]; subst.
+          destruct (typ_dec t0 t1); try solve [inversion HinterInsn]; subst.
+          destruct b; try solve [inversion HinterInsn].
+          destruct b.
+          inversion HinterInsn; subst.
+          eapply dsCall; eauto.
+            unfold lookupFdefViaGV.
+            rewrite <- HeqR0.
+            rewrite <- HeqR4.
+            rewrite <- HeqR1. auto.
+        
+          remember (lookupFdecViaIDFromProducts CurProducts0 i1) as R2.
+          destruct R2; simpl in HinterInsn;
+            try solve [inversion HinterInsn].
+            destruct f. destruct f.
+            destruct (id_dec i1 i2); try solve [inversion HinterInsn]; subst.
+            destruct (typ_dec t0 t1); try solve [inversion HinterInsn]; subst.
+            remember (callExternalFunction Mem0 i2 (params2GVs CurTargetData0 p lc Globals0)) as R3.
+            destruct R3.
+            inversion HinterInsn; subst.
+            eapply dsExCall; eauto.
+              unfold lookupExFdecViaGV.
+              rewrite <- HeqR0.
+              rewrite <- HeqR4.
+              rewrite <- HeqR1. eauto.
+Qed.
+
+
+
